opentheory/examples/stream.ml
@@ -16,4 +16,14 @@ export_thm stream_rep_abs;;
 
 let stream_tybij = CONJ stream_abs_rep stream_rep_abs;;
 
+let shd_def = new_definition
+  `!s : A stream. shd s = dest_stream s 0`;;
+
+export_thm shd_def;;
+
+let stl_def = new_definition
+  `!s : A stream. stl s = mk_stream (\n. dest_stream s (SUC n))`;;
+
+export_thm stl_def;;
+
 logfile_end ();;
